SemiTyped.v
@@ -1,0 +1,119 @@
+Require Import Arith.
+Require Import List.
+Import ListNotations.
+Open Scope list_scope.
+Require Import Program.
+Require Import Contexts.
+
+
+(* SYNTAX *)
+
+Inductive Pat : WType -> Set :=
+| unit  : Pat One
+| qubit : Pat Qubit
+| bit   : Pat Bit
+| pair  : forall {w1 w2}, Pat w1 -> Pat w2 -> Pat (Tensor w1 w2)
+.
+
+Inductive Unitary : WType -> Set := 
+  | H : Unitary Qubit 
+  | σx : Unitary Qubit
+  | σy : Unitary Qubit
+  | σz : Unitary Qubit
+  | CNOT : Unitary (Qubit ⊗ Qubit)
+  | control : forall {W} (U : Unitary W), Unitary (Qubit ⊗ W) 
+  | bit_control : forall {W} (U : Unitary W), Unitary (Bit ⊗ W) 
+  | transpose : forall {W} (U : Unitary W), Unitary W.
+Inductive Gate : WType -> WType -> Set := 
+  | U : forall {W} (u : Unitary W), Gate W W
+  | init0 : Gate One Qubit
+  | init1 : Gate One Qubit
+  | new0 : Gate One Bit
+  | new1 : Gate One Bit
+  | meas : Gate Qubit Bit
+  | discard : Gate Bit One.
+
+
+Inductive Circuit : WType -> Set :=
+| output : forall {w}, Pat w -> Circuit w
+| gate   : forall {w1 w2 w},
+           Gate w1 w2 -> Pat w1 -> Pat w2 -> Circuit w -> Circuit w
+| lift   : forall {w w'}, Pat w -> (interpret w -> Circuit w') -> Circuit w'
+.
+
+Fixpoint compose {W} (c : Circuit W) : forall {W'},
+                             (Pat W -> Circuit W') -> Circuit W' :=
+  match c with
+  | output p       => fun _ f => f p
+  | gate g p1 p2 k => fun _ f => gate g p1 p2 (compose k f)
+  | lift p g       => fun _ f => lift p (fun p' => compose (g p') f)
+  end.
+
+
+(* TYPING *) 
+
+Definition Merge (Γ1 Γ2 Γ : Ctx) := Γ1 ⋓ Γ2 = Γ.
+
+Inductive WF_Pat : forall {W}, Ctx -> Pat W -> Set :=
+| wf_unit  : WF_Pat [] unit
+| wf_qubit : forall {x Γ}, SingletonCtx x Qubit Γ -> WF_Pat Γ qubit
+| wf_bit   : forall {x Γ}, SingletonCtx x Bit Γ -> WF_Pat Γ bit
+| wf_pair  : forall {Γ1 Γ2 Γ : Ctx} {W1 W2} (p1 : Pat W1) (p2 : Pat W2), 
+             Merge Γ1 Γ2 Γ ->
+             WF_Pat Γ1 p1 -> WF_Pat Γ2 p2 -> WF_Pat Γ (pair p1 p2)
+.
+             
+Inductive WF_Circuit : forall {W}, Ctx -> Circuit W -> Set :=
+| wf_output : forall {W} (p : Pat W) {Γ},
+              WF_Pat Γ p ->
+              WF_Circuit Γ (output p)
+| wf_gate   : forall {W1 W2 W} {g : Gate W1 W2} 
+                     {p1 : Pat W1} {p2 : Pat W2} {c : Circuit W}
+                     {Γ1 Γ Γ1' Γ2 Γ2'},
+              Merge Γ1 Γ Γ1' -> Merge Γ2 Γ Γ2' ->
+              WF_Pat Γ1 p1 ->
+              WF_Pat Γ2 p2 ->
+              WF_Circuit Γ2' c ->
+              WF_Circuit Γ1' (gate g p1 p2 c)
+| wf_lift   : forall {W W'} {p : Pat W} {f : interpret W -> Circuit W'}
+                     {Γ Γ' Γ''},
+              Merge Γ Γ' Γ'' ->
+              WF_Pat Γ p ->
+              (forall (x : interpret W), WF_Circuit Γ' (f x)) ->
+              WF_Circuit Γ'' (lift p f)
+.
+
+
+
+(* should not be necessary for checking examples *)
+
+Lemma wf_compose : forall {W W'} {Γ Γ1 Γ1'} 
+                          (c : Circuit W) (f : Pat W -> Circuit W'),
+      Merge Γ1 Γ Γ1' -> 
+      WF_Circuit Γ1 c -> 
+      (forall (p : Pat W){Γ2 Γ2'}, Merge Γ2 Γ Γ2' -> WF_Pat Γ2 p -> WF_Circuit Γ2' (f p) ) ->
+      WF_Circuit Γ1' (compose c f).
+Admitted.
+(*
+Proof.
+  intros W W' Γ Γ1 Γ1' c f pf_merge wf_c.
+  revert W' Γ Γ1' f pf_merge.
+  induction wf_c; intros W0 Ω Ω1' h pf_merge H; simpl.
+  - eapply H; eauto.
+  - econstructor; [ | | eauto | eauto | ].
+    Focus 3. eapply IHwf_c; [ | eauto]. 
+      unfold Merge in *. admit (*?*).
+    * unfold Merge in *. 
+      assert (H0 : Γ1 ⋓ (Γ ⋓ Ω) = Ω1'). admit.
+      destruct (merge_valid _ _ _ H0).  destruct s; destruct s0. 
+      rewrite e0 in H0. exact H0.
+
+rewrite <- pf_merge at (Valid Ω1'). instantiate (0:=Γ ⋓ Ω).
+
+rewrite <- pf_merge at 2.
+
+Ω1' = Γ1' ⋓ Ω = Γ1 ⋓ Γ ⋓ Ω
+    *
+  - 
+  -
+*)
